theories/typing/uninit.v
@@ -1,0 +1,24 @@
+From lrust.typing Require Export type.
+From lrust.typing Require Import product.
+
+Section uninit.
+  Context `{typeG Σ}.
+
+  Program Definition uninit_1 : type :=
+    {| st_own tid vl := ⌜length vl = 1%nat⌝%I |}.
+  Next Obligation. done. Qed.
+
+  Definition uninit (n : nat) : type :=
+    Π (replicate n uninit_1).
+
+  Lemma eqtype_uninit_product E L ns :
+    eqtype E L (uninit (foldr plus 0%nat ns)) (Π(uninit <$> ns)).
+  Proof.
+    induction ns as [|n ns IH]. done.
+    rewrite /= /uninit replicate_plus (eqtype_prod_flatten E L []).
+    induction n. done. rewrite /product /=. by f_equiv.
+  Qed.
+
+  Lemma uninit_sz n : ty_size (uninit n) = n.
+  Proof. induction n. done. simpl. by f_equal. Qed.
+End uninit.
